Stlc/LemmasEvaluation.v
@@ -1,30 +1,232 @@
 Require Export Stlc.SpecSyntax.
 Require Export Stlc.SpecEvaluation.
 Require Export Stlc.LemmasSyntaxBasic.
+Require Export Coq.Program.Tactics.
 
-Lemma evalPlusToStar {t t'} : evalPlus t t' -> evalStar t t'.
+(* ** Evaluation contexts *)
+Lemma ectx_cat (C₁ C₂: PCtx) :
+  ECtx C₁ → ECtx C₂ → ECtx (pctx_cat C₁ C₂).
 Proof.
-  induction 1; apply rt1n_trans with y; eauto using clos_refl_trans_1n.
-Qed.
-      
-Lemma cycles_dont_terminate_help {t t'} : evalStar t' t -> evalPlus t t -> ~Terminating t'.
-Proof.
-  unfold not.
-  intros tptot ttot term.
-  depind term.
-  depind tptot.
-  * depind ttot.
-    + exact (H1 x H (rt1n_refl Tm eval x)).
-    + refine (H1 y H _). 
-      apply evalPlusToStar; assumption.
-  * apply H1 with y; assumption.
+  induction C₂; simpl; intros; destruct_conjs; auto.
 Qed.
 
-Lemma cycles_dont_terminate {t} : evalPlus t t -> ~Terminating t.
+Lemma evalstar_ctx C t t' (eC: ECtx C) :
+  t -->* t' → pctx_app t C -->* pctx_app t' C.
+Proof. induction 1; eauto using eval with eval. Qed.
+
+Lemma evalplus_ctx C t t' (eC: ECtx C) :
+  t -->+ t' → pctx_app t C -->+ pctx_app t' C.
+Proof. induction 1; eauto using eval with eval. Qed.
+
+
+(* ** Transitive and transitive-reflexive closure *)
+Lemma evalPlusToStar {t t'} : t -->+ t' -> t -->* t'.
+Proof. induction 1; eauto with eval. Qed.
+
+Lemma evalStarPlusToPlus {t t' t''} :
+  t -->* t' → t' -->+ t'' → t -->+ t''.
+Proof. induction 1; eauto with eval. Qed.
+
+Lemma evalPlusStepToPlus {t t' t''} :
+  t -->+ t' → t' --> t'' → t -->+ t''.
+Proof. induction 1; eauto with eval. Qed.
+
+Lemma evalPlusStarToPlus {t t' t''} :
+  t -->+ t' → t' -->* t'' → t -->+ t''.
+Proof. induction 2; eauto using evalPlusStepToPlus with eval. Qed.
+
+Lemma inversion_evalStar {t t'} :
+  t -->* t' → t = t' ∨ (t -->+ t').
+Proof. inversion 1; eauto using evalPlusStarToPlus with eval. Qed.
+
+
+(* Termination and divergene *)
+Lemma inversion_termination_app₁ {t₁ t₂} :
+  (app t₁ t₂)⇓ → t₁⇓.
 Proof.
-  apply cycles_dont_terminate_help; constructor.
+  intro nr. depind nr.
+  constructor; intros.
+  eapply H0; eauto.
+  eapply (eval_ctx (papp₁ phole t₂)); simpl; eauto.
 Qed.
 
+Lemma inversion_termination_app₂ {t₁ t₂} :
+  Value t₁ → (app t₁ t₂)⇓ → t₂⇓.
+Proof.
+  intros v₁ nr.
+  depind nr.
+  constructor; intros.
+  eapply H0; eauto.
+  eapply (eval_ctx (papp₂ t₁ phole)); simpl; eauto.
+Qed.
+
+(* Lemma inversion_termination_app₂' {t₁ τ₁ t₂} : *)
+(*   ⟪ empty ⊢ t₁ : τ₁ ⟫ → (app t₁ t₂)⇓ → t₂⇓. *)
+(* Proof. *)
+(*   intros wt₁ nr. *)
+(*   destruct (termination_value wt₁) as (t₁' & ? & ?). *)
+(*   eapply (inversion_termination_app₁ nr). *)
+(*   eapply inversion_termination_app₂; eauto. *)
+(*   assert (app t₁ t₂ -->* app t₁' t₂) *)
+(*     by (eapply (evalstar_ctx (papp₁ phole t₂)); simpl; auto). *)
+(*   eapply (termination_closed_under_evalstar H1); auto. *)
+(* Qed. *)
+
+Lemma inversion_termination_ite₁ {t₁ t₂ t₃} :
+  (ite t₁ t₂ t₃)⇓ → t₁⇓.
+Proof.
+  intro nr. depind nr.
+  constructor; intros.
+  eapply H0; eauto.
+  eapply (eval_ctx (pite₁ phole t₂ t₃)); simpl; eauto.
+Qed.
+
+Lemma inversion_termination_pair₁ {t₁ t₂} :
+  (pair t₁ t₂)⇓ → t₁⇓.
+Proof.
+  intro nr. depind nr.
+  constructor; intros.
+  eapply H0; eauto.
+  eapply (eval_ctx (ppair₁ phole t₂)); simpl; eauto.
+Qed.
+
+Lemma inversion_termination_pair₂ {t₁ t₂} :
+  Value t₁ → (pair t₁ t₂)⇓ → t₂⇓.
+Proof.
+  intros v₁ nr.
+  depind nr.
+  constructor; intros.
+  eapply H0; eauto.
+  eapply (eval_ctx (ppair₂ t₁ phole)); simpl; eauto.
+Qed.
+
+Lemma inversion_termination_proj₁ {t} :
+  (proj₁ t)⇓ → t⇓.
+Proof.
+  intro nr. depind nr.
+  constructor; intros.
+  eapply H0; eauto.
+  eapply (eval_ctx (pproj₁ phole)); simpl; eauto.
+Qed.
+
+Lemma inversion_termination_proj₂ {t} :
+  (proj₂ t)⇓ → t⇓.
+Proof.
+  intro nr. depind nr.
+  constructor; intros.
+  eapply H0; eauto.
+  eapply (eval_ctx (pproj₂ phole)); simpl; eauto.
+Qed.
+
+Lemma inversion_termination_inl {t} :
+  (inl t)⇓ → t⇓.
+Proof.
+  intro nr. depind nr.
+  constructor; intros.
+  eapply H0; eauto.
+  eapply (eval_ctx (pinl phole)); simpl; eauto.
+Qed.
+
+Lemma inversion_termination_inr {t} :
+  (inr t)⇓ → t⇓.
+Proof.
+  intro nr. depind nr.
+  constructor; intros.
+  eapply H0; eauto.
+  eapply (eval_ctx (pinr phole)); simpl; eauto.
+Qed.
+
+Lemma inversion_termination_caseof₁ {t₁ t₂ t₃} :
+  (caseof t₁ t₂ t₃)⇓ → t₁⇓.
+Proof.
+  intro nr. depind nr.
+  constructor; intros.
+  eapply H0; eauto.
+  eapply (eval_ctx (pcaseof₁ phole t₂ t₃)); simpl; eauto.
+Qed.
+
+Lemma inversion_termination_seq₁ {t₁ t₂} :
+  (seq t₁ t₂)⇓ → t₁⇓.
+Proof.
+  intro nr. depind nr.
+  constructor; intros.
+  eapply H0; eauto.
+  eapply (eval_ctx (pseq₁ phole t₂)); simpl; eauto.
+Qed.
+
+Lemma inversion_termination_fixt {τ₁ τ₂ t} :
+  (fixt τ₁ τ₂ t)⇓ → t⇓.
+Proof.
+  intro nr. depind nr.
+  constructor; intros.
+  eapply H0; eauto.
+  eapply (eval_ctx (pfixt τ₁ τ₂ phole)); simpl; eauto.
+Qed.
+
+Lemma inversion_termination_evalcontext :
+  ∀ C t, ECtx C → Terminating (pctx_app t C) → Terminating t.
+Proof.
+  induction C; crush; destruct_conjs;
+  try match goal with
+        | [ H: False |- _ ] => destruct H
+      end.
+  - eauto using inversion_termination_app₁.
+  - eauto using inversion_termination_app₂.
+  - eauto using inversion_termination_ite₁.
+  - eauto using inversion_termination_pair₁.
+  - eauto using inversion_termination_pair₂.
+  - eauto using inversion_termination_proj₁.
+  - eauto using inversion_termination_proj₂.
+  - eauto using inversion_termination_inl.
+  - eauto using inversion_termination_inr.
+  - eauto using inversion_termination_caseof₁.
+  - eauto using inversion_termination_seq₁.
+  - eauto using inversion_termination_fixt.
+Qed.
+
+Lemma termination_closed_under_evalplus {t t'} :
+  t -->+ t' → t⇓ → t'⇓.
+Proof. intros e m; induction e; inversion m; auto. Qed.
+
+Lemma termination_closed_under_evalstar {t t'} :
+  t -->* t' → t⇓ → t'⇓.
+Proof.
+  intros e; destruct (inversion_evalStar e); subst;
+    eauto using termination_closed_under_evalplus.
+Qed.
+
+Corollary divergence_closed_under_eval {t t'} :
+  t --> t' → t'⇑ → t⇑.
+Proof. eauto using TerminatingD with eval. Qed.
+
+Corollary divergence_closed_under_evalplus {t t'} :
+  t -->+ t' → t'⇑ → t⇑.
+Proof. eauto using termination_closed_under_evalplus. Qed.
+
+Corollary divergence_closed_under_evalstar {t t'} :
+  t -->* t' → t'⇑ → t⇑.
+Proof. eauto using termination_closed_under_evalstar. Qed.
+
+Corollary divergence_closed_under_evalcontex t :
+  t⇑ → ∀ p, ECtx p → (pctx_app t p)⇑.
+Proof. eauto using inversion_termination_evalcontext. Qed.
+
+(* Stronger induction principle *)
+Lemma Terminating_ind' (P: Tm → Prop)
+ (step: ∀ t,
+   (∀ t', t -->+ t' → t'⇓) →
+   (∀ t', t -->+ t' → P t') → P t) :
+  ∀ t, t⇓ → P t.
+Proof.
+  pose proof @termination_closed_under_evalplus.
+  intros t m.
+  apply step; eauto.
+  induction m; inversion 1; eauto.
+Qed.
+
+Lemma cycles_dont_terminate {t} :
+  t -->+ t → t⇑.
+Proof. induction 2 using Terminating_ind'; eauto. Qed.
 
 (* Local Variables: *)
 (* coq-load-path: (("." "Stlc")) *)
